Kue/Format.lean
@@ -158,6 +158,7 @@ mutual
           ++ formatValueWithFuel fuel right
     | _, .ref label => label
     | _, .refId id => s!"@{id.depth}.{id.index}"
+    | _, .thisStruct => "@self"
     | fuel + 1, .selector base label =>
         formatValueWithFuel fuel base ++ "." ++ formatFieldLabel label
     | fuel + 1, .index base key =>
