testdata/cue/value_aliases.cue
@@ -1,0 +1,14 @@
+#Secret: Self={
+	#name: "tls"
+	data:  Self.#name
+}
+
+aliased: X={
+	greeting: "hi"
+	echo:     X.greeting
+}
+
+nestedSelf: Self={
+	port: 8080
+	inner: lo: Self.port
+}
